Proofs.v
@@ -1,6 +1,30 @@
 From Licenta Require Import Semantics.
 From Licenta Require Import Syntax.
-From Licenta Require Import Unification_solver.
+From Licenta Require Import Unification_solver2.
 
-Check (Sbottom = Prop).
-Check (solver unif_probl1).
+Theorem apply_conflict_up_different: forall (u_p : unification_problem),
+  ~(check_conflict_and_deliver u_p = TError) /\ ~(u_p = Ubottom) ->
+  ~(u_p = occurs_check (mtp_to_tp (check_conflict_and_deliver u_p)) u_p).
+Proof.
+  intros. destruct H. induction u_p.
+  - simpl. apply H0.
+  - destruct ((check_conflict_and_deliver (Uset l))).
+    -- contradiction.
+    -- simpl. unfold occurs_check. unfold remove_conflict_term_pair. apply H0.
+Qed.
+
+Theorem progress'' : forall (m_u_p: maybe_unification_problem),
+  ~(m_u_p = UError) /\
+  ~(m_u_p = UP Ubottom) /\ ~(unification_problem_in_solved_form (mup_to_up m_u_p) = true) ->
+  (exists (m_u_p' : maybe_unification_problem), (apply_one_step' m_u_p = m_u_p') /\ ~(m_u_p = m_u_p')).
+Proof.
+  intros. destruct H. destruct H0. exists (apply_one_step' m_u_p). split.
+  - reflexivity.
+  - destruct m_u_p.
+    -- contradiction.
+    -- simpl.  destruct u_p.
+      --- contradiction.
+      --- simpl in H1. destruct (unification_problem_in_solved_form (Uset l)).
+        ---- contradiction.
+        ---- destruct (check_conflict_and_deliver (Uset l)).
+          2 : { apply apply_conflict_up_different.
